\documentclass{article}
%\usepackage[left=3cm,right=3cm,top=0cm,bottom=2cm]{geometry} % page settings
\usepackage[a4paper, margin=0.1in]{geometry}
\usepackage{amsmath} % provides many mathematical environments & tools
\setlength{\parindent}{0mm}
\begin{document}

\title{Math}
\author{Nicolas Schmidt}
\date{\today}
\maketitle

\subsection*{I Dunno 1.2.4}


Assume $$ f(c)=f(a+b) = f(a)f(b) $$ for all real numbers a and b\\

$ f(0)=f(0+0) = f(0)f(0) $ implies that $ f(0) = 1 $ or $f(0)=0$\\

if $f(0) = 0$ then $f(0) = f(a-a) = f(a)f(-a) = 0$ which means that $f(a) = 0$ for all a \\

if $f(0) = 1$ then 

$$f(0) = f(a-a) = f(a)f(-a) => f(-a) = (f(a))-1 = 1/f(a) $$

$$f(na)=nf(a)$$

$$f(a)=f(nb) = (f(b))n$$

## Cross multiplication rule

$$(x+a)(x+b) = x^2 + (a+b)x + ab \\
$$

## Quadratic Equation

$$ax^2 + bx + c = 0 $$

$$ a ( x^2 + bx/a ) + c = 0 $$
a ( x^2 + 2 bx/2a + (b/2a)^2  - (b/2a)^2  ) + c = 0$$
a ( x^2 + 2 bx/2a + (b/2a)^2   ) - b^2/4a + c = 0$$
a ( x + b/2a ) ^2 - b^2/4a + c = 0$$
x = -b/2a \pm \sqrt{ b^2/4a^2 - c/a }$$

## Imaginary Numbers

$$(ai + bj) ( ci + dj ) = (ac + bd) + (ad -bc) ij$$

## Geometric Algebra

Orthogonal vectors anticommute

x and y are unit vectors (0,1) and (1,0)

$$(ax+by)(cx+dy) = (ac+bd) + (ad-bc)xy \\
xx=1\\
yx=-xy$$

$$(xy)^2 = xyxy = -xyyx = -1$$

A product of two orthogonal vectors is isomorphic to the imaginary number.

## Parabolic Arc

$$x = vt \cos\theta \\
y = vt \sin\theta + g t^2 / 2 \\

$$

$$y = \frac {x \sin\theta } {\cos\theta } + \frac{g}{2}\bigg(\frac{x}{v\cos\theta}\bigg)^2$$

$$y = x \tan\theta + \frac{gx^2}{2v^2} (1+\tan^2\theta) $$

Which angle gives maximum distance x? Find angle where $dx/d\theta = 0$ .  

$$\frac{gx^2}{2v^2} (1+\tan^2\theta) + x \tan\theta -y = 0$$

$$x = \frac{ -\tan\theta \pm \sqrt{\tan^2\theta - 4\frac{gx^2}{2v^2}(1+\tan^2\theta)(-y) } } { \frac{g}{v^2} (1+\tan^2\theta) }$$

Assume that g=v=1 and y = 0

$$x = \frac{ -\tan\theta \pm \sqrt{\tan^2\theta} } { (1+\tan^2\theta) }$$

$$x = 0, \frac{ -2\tan\theta } { (1+\tan^2\theta) }$$

$$\frac{gx^2}{2v^2} \tan^2\theta + x \tan\theta  + \bigg(\frac{gx^2}{2v^2} -y \bigg) = 0$$




\end{document}